Add definitions of strong permutative equality for named tensorlists and hypergraphs, and prove semantic correctness

theories/GraphCore/SPGraphRewriting.v
@@ -7,179 +7,93 @@ Require Import Aux_pos.
 
 (* An implementation of double pushout (DPO) rewriting *)
 
-(* 
+
 Local Open Scope nat_scope.
 
 Section DPO.
 
   Context {T : Type}.
 
-  Fixpoint propogate_subst {n} (ps : vec (positive * positive) n) : vec (positive * positive) n :=
-  match n, ps with
-  | 0, _ => [#]
-  | (S k), _ =>
-    let (p, p') := Vector.hd ps in
-    let ps' := Vector.tl ps in
-      (p, p') ::: propogate_subst (vmap (prod_map {[p := p']} {[p := p']}) ps')
-  end.
-
-  Fixpoint subst_by_vec {n} (ps : vec (positive * positive) n) (p : positive) : positive :=
-    match ps with
-    | [#] => p
-    | (a, b) ::: ps' => subst_by_vec ps' ({[a := b]} p)
-    end.
 
   (* Reserved Notation "tgl ; tgr" (at level 50). *)
-  Definition compose_safe {n m o} (tgl : CospanHyperGraph T n m) (tgr : CospanHyperGraph T m o) : CospanHyperGraph T n o :=
+  Definition spcompose_safe {n m o} (tgl : CospanSPHyperGraph T n m) (tgr : CospanSPHyperGraph T m o) : CospanSPHyperGraph T n o :=
     let connected_substs :=
-        propogate_subst (vzip (vmap (bcons false) tgl.(outputs)) (vmap (bcons true) tgr.(inputs))) in
-     relabel_graph (subst_by_vec connected_substs) ((vmap (bcons false) tgl.(inputs)) ->
-      hg_add_vertices (tgl.(hedges) ⊎ tgr.(hedges)) (list_to_set (vmap (bcons true) tgr.(inputs))) <- (vmap (bcons true) tgr.(outputs))).
+        propogate_subst (vzip (vmap (bcons false) tgl.(spoutputs)) (vmap (bcons true) tgr.(spinputs))) in
+     relabel_spgraph (subst_by_vec connected_substs) ((vmap (bcons false) tgl.(spinputs)) ->
+      sphg_add_vertices (tgl.(sphedges) ⊎ tgr.(sphedges)) (list_to_set (vmap (bcons true) tgr.(spinputs))) <- (vmap (bcons true) tgr.(spoutputs))).
 
-  Definition compose {n m o} (tgl : CospanHyperGraph T n m) (tgr : CospanHyperGraph T m o) : CospanHyperGraph T n o :=
-    let connected_substs := propogate_subst (vzip (tgl.(outputs)) (tgr.(inputs))) in
-    relabel_graph (subst_by_vec connected_substs)
-      (tgl.(inputs) ->
-        hg_add_vertices (tgl.(hedges) ∪ tgr.(hedges)) (list_to_set tgr.(inputs))
-          <- tgr.(outputs)).
+  Definition spcompose {n m o} (tgl : CospanSPHyperGraph T n m) (tgr : CospanSPHyperGraph T m o) : CospanSPHyperGraph T n o :=
+    let connected_substs := propogate_subst (vzip (tgl.(spoutputs)) (tgr.(spinputs))) in
+    relabel_spgraph (subst_by_vec connected_substs)
+      (tgl.(spinputs) ->
+        sphg_add_vertices (tgl.(sphedges) ∪ tgr.(sphedges)) (list_to_set tgr.(spinputs))
+          <- tgr.(spoutputs)).
 
-  Definition compose_unsafe {n m o} (tgl : CospanHyperGraph T n m) (tgr : CospanHyperGraph T m o) : CospanHyperGraph T n o :=
-    tgl.(inputs) ->  hg_add_vertices (tgl.(hedges) ∪ tgr.(hedges)) (list_to_set (tgr.(inputs))) <- tgr.(outputs).
+  Definition spcompose_unsafe {n m o} (tgl : CospanSPHyperGraph T n m) (tgr : CospanSPHyperGraph T m o) : CospanSPHyperGraph T n o :=
+    tgl.(spinputs) ->  sphg_add_vertices (tgl.(sphedges) ∪ tgr.(sphedges)) (list_to_set (tgr.(spinputs))) <- tgr.(spoutputs).
 
-Lemma compose_safe_to_compose {n m o}
-  (tgl : CospanHyperGraph T n m) (tgr : CospanHyperGraph T m o) :
-  compose_safe tgl tgr = compose
-    (reindex_graph (bcons false) (relabel_graph (bcons false) tgl))
-    (reindex_graph (bcons true) (relabel_graph (bcons true) tgr)).
+Lemma spcompose_safe_to_spcompose {n m o}
+  (tgl : CospanSPHyperGraph T n m) (tgr : CospanSPHyperGraph T m o) :
+  spcompose_safe tgl tgr = spcompose
+    (reindex_spgraph (bcons false) (relabel_spgraph (bcons false) tgl))
+    (reindex_spgraph (bcons true) (relabel_spgraph (bcons true) tgr)).
 Proof.
   reflexivity.
 Qed.
 
-Lemma subst_by_vec_id {n} : forall v : vec positive n, forall p : positive,
-  subst_by_vec (propogate_subst (vzip_with pair v v)) p = p.
-Proof.
-  induction v.
-  - easy.
-  - intros.
-    simpl.
-    rewrite Vector.map_ext with (g:=(λ x : _, x)).
-    + rewrite Vector.map_id.
-      rewrite fn_lookup_singleton_case.
-      case_decide; subst; auto.
-    + intros.
-      destruct a.
-      simpl.
-      rewrite 2 fn_lookup_singleton_case.
-      case_decide; case_decide; subst; reflexivity.
-Qed.
 
-Lemma compose_to_compose_unsafe {n m o} (tgl : CospanHyperGraph T n m) (tgr : CospanHyperGraph T m o) :
-  tgl.(outputs) = tgr.(inputs) ->
-  compose tgl tgr = compose_unsafe tgl tgr.
+Lemma spcompose_to_spcompose_unsafe {n m o} (tgl : CospanSPHyperGraph T n m) (tgr : CospanSPHyperGraph T m o) :
+  tgl.(spoutputs) = tgr.(spinputs) ->
+  spcompose tgl tgr = spcompose_unsafe tgl tgr.
 Proof.
   intros.
-  unfold compose.
+  unfold spcompose.
   rewrite H.
-  unfold relabel_graph.
+  unfold relabel_spgraph.
   rewrite Vector.map_ext with (g:=(λ x : _, x)).
   rewrite Vector.map_id.
   simpl.
   rewrite Vector.map_ext with (g:=(λ x : _, x)).
   rewrite Vector.map_id.
   simpl.
-  rewrite relabel_hg_id'.
+  rewrite relabel_sphg_id'.
   reflexivity.
   all: apply subst_by_vec_id.
 Qed.
 
 
-Lemma relabel_hg_union f (hg hg' : HyperGraph T) :
-  relabel_hg f (hg ∪ hg') =
-  relabel_hg f hg ∪ relabel_hg f hg'.
+Lemma relabel_sphg_union f (sphg sphg' : SPHyperGraph T) :
+  relabel_sphg f (sphg ∪ sphg') =
+  relabel_sphg f sphg ∪ relabel_sphg f sphg'.
 Proof.
-  apply hg_ext; cbn.
+  apply sphg_ext; cbn.
   - now rewrite map_fmap_union.
   - now rewrite set_map_union_L.
 Qed.
 
-Lemma reindex_hg_union f `{Hf : !Inj eq eq f} (hg hg' : HyperGraph T) :
-  reindex_hg f (hg ∪ hg') =
-  reindex_hg f hg ∪ reindex_hg f hg'.
+Lemma reindex_sphg_union f `{Hf : !Inj eq eq f} (sphg sphg' : SPHyperGraph T) :
+  reindex_sphg f (sphg ∪ sphg') =
+  reindex_sphg f sphg ∪ reindex_sphg f sphg'.
 Proof.
-  apply hg_ext; cbn.
+  apply sphg_ext; cbn.
   - apply (kmap_union _).
   - done.
 Qed.
 
 
 
-Lemma apply_fn_lookup_singleton `{EqDecision A, EqDecision B}
-  (f : A -> B) `{Hf : !Inj eq eq f} (a b c : A) :
-  f ({[a := b]} c) = {[f a := f b]} (f c).
-Proof.
-  rewrite fn_lookup_singleton_case.
-  case_decide as Hac.
-  - subst.
-    now rewrite fn_lookup_singleton.
-  - now rewrite fn_lookup_singleton_ne by now intros ?%(inj f).
-Qed.
-
-Lemma propogate_subst_vmap {n} (fl : positive -> positive)
-  `{Hfl : !Inj eq eq fl} (v : vec _ n) :
-  (* v.*1 ## v.*2 -> *)
-  propogate_subst (vmap (prod_map fl fl) v) =
-  vmap (prod_map fl fl) (propogate_subst v).
-Proof.
-  revert v; induction n as [|n IHn]; [refine (vec_0_inv _ _);done|
-    refine (vec_S_inv _ _)].
-  intros (p, q) v.
-  cbn.
-  (* intros Hdisj. *)
-  f_equal.
-  rewrite <- IHn.
-  f_equal.
-  apply vec_eq; intros i.
-  rewrite 2 Vector.map_map, 2 vlookup_map.
-  destruct (v !!! i) as (pi, qi).
-  cbn.
-  now rewrite 2 (apply_fn_lookup_singleton fl).
-Qed.
-
-Lemma susbt_by_vec_propogate_helper n i o
-  (insl outsl : vec positive n) (p' : positive) :
-  subst_by_vec (propogate_subst
-       (vzip_with pair (vmap {[o := i]} outsl) (vmap {[o := i]} insl))) p' =
-  subst_by_vec (propogate_subst
-      (vmap (prod_map {[o := i]} {[o := i]}) (vzip_with pair outsl insl))) p'.
-Proof.
-  revert i o insl outsl p'.
-  induction n; intros i o;
-  [do 2 refine (vec_0_inv _ _); done|].
-  refine (vec_S_inv _ _).
-  intros i' insl.
-  refine (vec_S_inv _ _).
-  intros o' outsl p.
-  cbn.
-  rewrite <- vzip_map.
-  rewrite IHn.
-  f_equal.
-  f_equal.
-  rewrite vzip_map.
-  done.
-Qed.
-
-Lemma inputs_add_top_loops {n m m'}
-  (tg : CospanHyperGraph T (n + m) (n + m')) :
-  (add_top_loops tg).(inputs) =
+Lemma spinputs_spadd_top_loops {n m m'}
+  (tg : CospanSPHyperGraph T (n + m) (n + m')) :
+  (spadd_top_loops tg).(spinputs) =
   vmap (subst_by_vec (propogate_subst
-    (vzip (vsplitl tg.(outputs))
-      (vsplitl tg.(inputs)))))
-      (vsplitr tg.(inputs)).
+    (vzip (vsplitl tg.(spoutputs))
+      (vsplitl tg.(spinputs)))))
+      (vsplitr tg.(spinputs)).
 Proof.
   induction n; [cbn; now rewrite Vector.map_id|].
-  cbn [add_top_loops].
+  cbn [spadd_top_loops].
   rewrite IHn.
-  destruct tg as [hg ins outs].
+  destruct tg as [sphg ins outs].
   (* cbn in ins, outs. *)
   induction ins as [insl insr] using vec_add_inv.
   induction outs as [outsl outsr] using vec_add_inv.
@@ -197,18 +111,18 @@ Proof.
 Qed.
 
 
-Lemma outputs_add_top_loops {n m m'}
-  (tg : CospanHyperGraph T (n + m) (n + m')) :
-  (add_top_loops tg).(outputs) =
+Lemma spoutputs_spadd_top_loops {n m m'}
+  (tg : CospanSPHyperGraph T (n + m) (n + m')) :
+  (spadd_top_loops tg).(spoutputs) =
   vmap (subst_by_vec (propogate_subst
-    (vzip (vsplitl tg.(outputs))
-      (vsplitl tg.(inputs)))))
-      (vsplitr tg.(outputs)).
+    (vzip (vsplitl tg.(spoutputs))
+      (vsplitl tg.(spinputs)))))
+      (vsplitr tg.(spoutputs)).
 Proof.
   induction n; [cbn; now rewrite Vector.map_id|].
-  cbn [add_top_loops].
+  cbn [spadd_top_loops].
   rewrite IHn.
-  destruct tg as [hg ins outs].
+  destruct tg as [sphg ins outs].
   (* cbn in ins, outs. *)
   induction ins as [insl insr] using vec_add_inv.
   induction outs as [outsl outsr] using vec_add_inv.
@@ -225,48 +139,48 @@ Proof.
   apply susbt_by_vec_propogate_helper.
 Qed.
 
-Lemma hg_add_vertices_empty (hg : HyperGraph T) :
-  hg_add_vertices hg ∅ = hg.
+Lemma sphg_add_vertices_empty (sphg : SPHyperGraph T) :
+  sphg_add_vertices sphg ∅ = sphg.
 Proof.
-  apply hg_ext; [done|].
+  apply sphg_ext; [done|].
   cbn -[union].
   apply union_empty_l_L.
 Qed.
 
-Lemma hg_add_vertices_union (hg : HyperGraph T) vs vs' :
-  hg_add_vertices (hg_add_vertices hg vs) vs' =
-  hg_add_vertices hg (vs ∪ vs').
+Lemma sphg_add_vertices_union (sphg : SPHyperGraph T) vs vs' :
+  sphg_add_vertices (sphg_add_vertices sphg vs) vs' =
+  sphg_add_vertices sphg (vs ∪ vs').
 Proof.
-  apply hg_ext; [done|].
+  apply sphg_ext; [done|].
   cbn -[union].
   rewrite (union_assoc_L _).
   f_equal.
   apply union_comm_L.
 Qed.
 
-Lemma relabel_hg_add_vertices f (hg : HyperGraph T) vs :
-  relabel_hg f (hg_add_vertices hg vs) =
-  hg_add_vertices (relabel_hg f hg) (set_map f vs).
+Lemma relabel_sphg_add_vertices f (sphg : SPHyperGraph T) vs :
+  relabel_sphg f (sphg_add_vertices sphg vs) =
+  sphg_add_vertices (relabel_sphg f sphg) (set_map f vs).
 Proof.
-  apply hg_ext; [done|].
+  apply sphg_ext; [done|].
   cbn.
   now rewrite set_map_union_L.
 Qed.
 
 
-Lemma hedges_add_top_loops {n m m'}
-  (tg : CospanHyperGraph T (n + m) (n + m')) :
-  (add_top_loops tg).(hedges) =
-  relabel_hg (subst_by_vec (propogate_subst
-    (vzip (vsplitl tg.(outputs))
-      (vsplitl tg.(inputs)))))
-      (hg_add_vertices tg.(hedges)
-      (list_to_set (vsplitl tg.(inputs)))).
+Lemma sphedges_spadd_top_loops {n m m'}
+  (tg : CospanSPHyperGraph T (n + m) (n + m')) :
+  (spadd_top_loops tg).(sphedges) =
+  relabel_sphg (subst_by_vec (propogate_subst
+    (vzip (vsplitl tg.(spoutputs))
+      (vsplitl tg.(spinputs)))))
+      (sphg_add_vertices tg.(sphedges)
+      (list_to_set (vsplitl tg.(spinputs)))).
 Proof.
-  induction n; [cbn; now rewrite relabel_hg_id, hg_add_vertices_empty|].
-  cbn [add_top_loops].
+  induction n; [cbn; now rewrite relabel_sphg_id, sphg_add_vertices_empty|].
+  cbn [spadd_top_loops].
   rewrite IHn.
-  destruct tg as [hg ins outs].
+  destruct tg as [sphg ins outs].
   (* cbn in ins, outs. *)
   induction ins as [insl insr] using vec_add_inv.
   induction outs as [outsl outsr] using vec_add_inv.
@@ -276,10 +190,10 @@ Proof.
   rewrite 2 vsplitl_app.
   cbn -[union].
   rewrite 2 vsplitl_map, 2 vsplitl_app.
-  rewrite 4 relabel_hg_add_vertices, hg_add_vertices_union.
+  rewrite 4 relabel_sphg_add_vertices, sphg_add_vertices_union.
   f_equal.
-  - rewrite relabel_hg_compose.
-    apply relabel_hg_ext.
+  - rewrite relabel_sphg_compose.
+    apply relabel_sphg_ext.
     intros p; cbn.
     now rewrite susbt_by_vec_propogate_helper.
   - rewrite <- set_map_union_L.
@@ -292,55 +206,55 @@ Proof.
     apply susbt_by_vec_propogate_helper.
 Qed.
 
-Lemma add_top_loops_alt {n m m'}
-  (tg : CospanHyperGraph T (n + m) (n + m')) :
-  add_top_loops tg =
-  relabel_graph (subst_by_vec (propogate_subst
-    (vzip (vsplitl tg.(outputs))
-      (vsplitl tg.(inputs)))))
-    (vsplitr tg.(inputs) ->
-      hg_add_vertices tg.(hedges) (list_to_set (vsplitl tg.(inputs)))
-      <- vsplitr tg.(outputs)).
+Lemma spadd_top_loops_alt {n m m'}
+  (tg : CospanSPHyperGraph T (n + m) (n + m')) :
+  spadd_top_loops tg =
+  relabel_spgraph (subst_by_vec (propogate_subst
+    (vzip (vsplitl tg.(spoutputs))
+      (vsplitl tg.(spinputs)))))
+    (vsplitr tg.(spinputs) ->
+      sphg_add_vertices tg.(sphedges) (list_to_set (vsplitl tg.(spinputs)))
+      <- vsplitr tg.(spoutputs)).
 Proof.
-  apply cohg_ext.
-  - apply hedges_add_top_loops.
-  - apply inputs_add_top_loops.
-  - apply outputs_add_top_loops.
+  apply cosphg_ext.
+  - apply sphedges_spadd_top_loops.
+  - apply spinputs_spadd_top_loops.
+  - apply spoutputs_spadd_top_loops.
 Qed.
 
 
 
-Lemma compose_graphs_alt_aux_correct {n m o}
-  (tgl : CospanHyperGraph T n m) (tgr : CospanHyperGraph T m o) :
-  add_top_loops (swapped_stack_graphs_aux tgl tgr) =
-    compose tgl tgr.
+Lemma spcompose_spgraphs_alt_aux_correct {n m o}
+  (tgl : CospanSPHyperGraph T n m) (tgr : CospanSPHyperGraph T m o) :
+  spadd_top_loops (swapped_stack_spgraphs_aux tgl tgr) =
+    spcompose tgl tgr.
 Proof.
-  rewrite add_top_loops_alt.
+  rewrite spadd_top_loops_alt.
   cbn.
   rewrite 2 vsplitl_app, 2 vsplitr_app.
   reflexivity.
 Qed.
 
-Lemma compose_graphs_alt_correct {n m o}
-  (tgl : CospanHyperGraph T n m) (tgr : CospanHyperGraph T m o) :
-  add_top_loops (swapped_stack_graphs tgl tgr) =
-    compose_safe tgl tgr.
+Lemma spcompose_spgraphs_alt_correct {n m o}
+  (tgl : CospanSPHyperGraph T n m) (tgr : CospanSPHyperGraph T m o) :
+  spadd_top_loops (swapped_stack_spgraphs tgl tgr) =
+    spcompose_safe tgl tgr.
 Proof.
-  rewrite add_top_loops_alt.
+  rewrite spadd_top_loops_alt.
   cbn.
   rewrite 2 vsplitl_app, 2 vsplitr_app.
-  rewrite <- 2 reindex_relabel_hg.
+  rewrite <- 2 reindex_relabel_sphg.
   done.
 Qed.
 
 
-Lemma relabel_stack_graphs_aux {n m n' m'} (cohg : CospanHyperGraph T n m)
-  (cohg' : CospanHyperGraph T n' m') f :
-  relabel_graph f (stack_graphs_aux cohg cohg') =
-  stack_graphs_aux (relabel_graph f cohg) (relabel_graph f cohg').
+Lemma relabel_stack_spgraphs_aux {n m n' m'} (cosphg : CospanSPHyperGraph T n m)
+  (cosphg' : CospanSPHyperGraph T n' m') f :
+  relabel_spgraph f (stack_spgraphs_aux cosphg cosphg') =
+  stack_spgraphs_aux (relabel_spgraph f cosphg) (relabel_spgraph f cosphg').
 Proof.
-  apply cohg_ext.
-  - cbn; apply relabel_hg_union.
+  apply cosphg_ext.
+  - cbn; apply relabel_sphg_union.
   - cbn.
     now rewrite Vector.map_append.
   - cbn.
@@ -348,106 +262,60 @@ Proof.
 Qed.
 
 
-Lemma stack_graphs_relabel {n m n' m'} (cohg : CospanHyperGraph T n m)
-  (cohg' : CospanHyperGraph T n' m') ft fb :
-  stack_graphs (relabel_graph ft cohg) (relabel_graph fb cohg') =
-  relabel_graph (pos_map ft fb) (stack_graphs cohg cohg').
+Lemma stack_spgraphs_relabel {n m n' m'} (cosphg : CospanSPHyperGraph T n m)
+  (cosphg' : CospanSPHyperGraph T n' m') ft fb :
+  stack_spgraphs (relabel_spgraph ft cosphg) (relabel_spgraph fb cosphg') =
+  relabel_spgraph (pos_map ft fb) (stack_spgraphs cosphg cosphg').
 Proof.
-  unfold stack_graphs.
-  rewrite relabel_stack_graphs_aux.
-  rewrite 2 reindex_relabel_graph, 4 relabel_graph_compose.
+  unfold stack_spgraphs.
+  rewrite relabel_stack_spgraphs_aux.
+  rewrite 2 reindex_relabel_spgraph, 4 relabel_spgraph_compose.
   done.
 Qed.
 
-Lemma reindex_stack_graphs_aux {n m n' m'} (cohg : CospanHyperGraph T n m)
-  (cohg' : CospanHyperGraph T n' m') f `{Hf : !Inj eq eq f} :
-  reindex_graph f (stack_graphs_aux cohg cohg') =
-  stack_graphs_aux (reindex_graph f cohg) (reindex_graph f cohg').
+Lemma reindex_stack_spgraphs_aux {n m n' m'} (cosphg : CospanSPHyperGraph T n m)
+  (cosphg' : CospanSPHyperGraph T n' m') f `{Hf : !Inj eq eq f} :
+  reindex_spgraph f (stack_spgraphs_aux cosphg cosphg') =
+  stack_spgraphs_aux (reindex_spgraph f cosphg) (reindex_spgraph f cosphg').
 Proof.
-  apply cohg_ext; [|done..].
+  apply cosphg_ext; [|done..].
   cbn.
-  apply (reindex_hg_union _).
+  apply (reindex_sphg_union _).
 Qed.
 
-Lemma stack_graphs_reindex {n m n' m'} (cohg : CospanHyperGraph T n m)
-  (cohg' : CospanHyperGraph T n' m') ft fb 
+Lemma stack_spgraphs_reindex {n m n' m'} (cosphg : CospanSPHyperGraph T n m)
+  (cosphg' : CospanSPHyperGraph T n' m') ft fb 
   `{Hft : !Inj eq eq ft, Hfb : !Inj eq eq fb} :
-  stack_graphs (reindex_graph ft cohg) (reindex_graph fb cohg') =
-  reindex_graph (pos_map ft fb) (stack_graphs cohg cohg').
+  stack_spgraphs (reindex_spgraph ft cosphg) (reindex_spgraph fb cosphg') =
+  reindex_spgraph (pos_map ft fb) (stack_spgraphs cosphg cosphg').
 Proof.
-  unfold stack_graphs.
-  rewrite (reindex_stack_graphs_aux _ _ _).
-  rewrite 2 reindex_relabel_graph, 4 (reindex_graph_compose _ _).
+  unfold stack_spgraphs.
+  rewrite (reindex_stack_spgraphs_aux _ _ _).
+  rewrite 2 reindex_relabel_spgraph, 4 (reindex_spgraph_compose _ _).
   done.
 Qed.
 
-Lemma stack_graphs_isomorphic {n m n' m'} (cohg1 cohg1' : CospanHyperGraph T n m)
-  (cohg2 cohg2' : CospanHyperGraph T n' m') : 
-  isomorphic cohg1 cohg1' -> isomorphic cohg2 cohg2' ->
-  isomorphic (stack_graphs cohg1 cohg2) (stack_graphs cohg1' cohg2').
+Lemma stack_spgraphs_spisomorphic {n m n' m'} (cosphg1 cosphg1' : CospanSPHyperGraph T n m)
+  (cosphg2 cosphg2' : CospanSPHyperGraph T n' m') : 
+  spisomorphic cosphg1 cosphg1' -> spisomorphic cosphg2 cosphg2' ->
+  spisomorphic (stack_spgraphs cosphg1 cosphg2) (stack_spgraphs cosphg1' cosphg2').
 Proof.
-  intros (fv1 & fe1 & Hfv1 & Hfe1 & ->)%isomorphic_exists
-    (fv2 & fe2 & Hfv2 & Hfe2 & ->)%isomorphic_exists.
-  rewrite stack_graphs_relabel, (stack_graphs_reindex _ _ _ _).
-  apply (iso_relabel_reindex _ _ _).
+  intros (fv1 & fe1 & Hfv1 & Hfe1 & ->)%spisomorphic_exists
+    (fv2 & fe2 & Hfv2 & Hfe2 & ->)%spisomorphic_exists.
+  rewrite stack_spgraphs_relabel, (stack_spgraphs_reindex _ _ _ _).
+  apply (spiso_relabel_reindex _ _ _).
 Qed.
 
 
 
-Section Paths.
-
-  Context (H : HyperGraph T).
-
-  Definition successor (h h' : HyperEdge T) :=
-    exists p, In p (h.1.2) /\ In p (h'.2).
-
-  Definition predecessor (h h' : HyperEdge T) :=
-    exists p, In p (h'.1.2) /\ In p (h.2).
-
-  Lemma succ_pred_symm (h h' : HyperEdge T) :
-    successor h h' <-> predecessor h' h.
-  Proof.
-    split;
-      intros [x []];
-      exists x;
-      auto.
-  Qed.
-
-  Definition path (h h' : HyperEdge T) : Prop :=
-    (tc successor) h h'.
-
-  Definition pred_path (h h' : HyperEdge T) :=
-    (tc predecessor) h h'.
-
-  (* Definition path_pred_path_symm (h h' : HyperEdge T) :
-    path h h' <-> pred_path h' h.
-  Proof.
-    split.
-    intros.
-    - induction H0.
-      + apply tc_once.
-        now rewrite succ_pred_symm in H0.
-      +
-        rewrite IHtc.
-    - intros [x y | x y].
-      +  *)
-
-
-End Paths.
-
-Definition decompose_left {n m} (G : CospanHyperGraph T n m) (L : HyperGraph T) : CospanHyperGraph T n m :=
-  G.(inputs) -> {|
-    hyperedges := ∅;
-    hypervertices := ∅
-  |} <- G.(outputs).
 
 
 End DPO.
 
 
-Add Parametric Morphism {T n m n' m'} : (@stack_graphs T n m n' m') with signature 
-  isomorphic ==> isomorphic ==> isomorphic as stack_graphs_isomorphic_mor.
+Add Parametric Morphism {T n m n' m'} : (@stack_spgraphs T n m n' m') with signature 
+  spisomorphic ==> spisomorphic ==> spisomorphic as stack_spgraphs_spisomorphic_mor.
 Proof.
-  intros; now apply stack_graphs_isomorphic.
+  intros; now apply stack_spgraphs_spisomorphic.
 Qed.
-   *)
+  
