theories/GraphCore/SPTensorGraphGraph.v
@@ -1,0 +1,4 @@
+Require Import SPTensorGraph SPIsomorphismTesting SPGraphRewriting.
+Require Import TensorGraph GraphRewriting.
+
+
