theories/GraphCore/TensorGraphSP.v
@@ -1,0 +1,134 @@
+Require Import SetoidList SetoidPermutation.
+From stdpp Require Import fin_maps.
+Require Import TEPerm.
+Require Export TensorGraph TensorGraphExpr TensorGraphSemantics TensorGraphFacts.
+
+
+Lemma map_relation_to_dom' `{FinMap K M} {A} P (m1 m2 : M A) :
+  map_relation P (λ _ _, False) (λ _ _, False) m1 m2 ->
+  (forall j, is_Some (m1 !! j) <-> is_Some (m2 !! j)).
+Proof.
+  intros Hrel j.
+  specialize (Hrel j).
+  rewrite 2 is_Some_alt.
+  do 2 case_match; done.
+Qed.
+
+Lemma map_relation_to_map_to_list `{FinMap K M} {A} P (m1 m2 : M A) :
+  map_relation P (λ _ _, False) (λ _ _, False) m1 m2 ->
+  Forall2 (λ ka kb, ka.1 = kb.1 /\ P ka.1 ka.2 kb.2)
+    (map_to_list m1) (map_to_list m2).
+Proof.
+  revert m2; induction m1 as [|i a m1 Hm1i H1fst IHm1] using map_first_key_ind; intros m2 Hrel.
+  - replace m2 with (∅ :> M A); [now rewrite map_to_list_empty|].
+    symmetry.
+    apply map_empty.
+    intros i.
+    pose proof ((map_relation_to_dom' _ _ _ Hrel i).2) as Hsome.
+    rewrite lookup_empty in Hsome.
+    rewrite 2 is_Some_alt in Hsome.
+    now destruct (m2 !! i).
+  - specialize (map_relation_to_dom' _ _ _ Hrel) as Hdom'.
+    rewrite map_to_list_insert_first_key by done.
+    assert (H2fst : map_first_key m2 i). 1:{
+      revert H1fst.
+      now refine (map_first_key_dom' _ _ _ _).1.
+    }
+    assert (Hm2i : is_Some (m2 !! i)) by now rewrite <- Hdom', lookup_insert.
+    destruct Hm2i as [m2i Hm2i].
+    rewrite <- (insert_delete _ _ _ Hm2i) in Hrel |- *.
+    rewrite map_to_list_insert_first_key by
+      first [apply lookup_delete|now rewrite insert_delete].
+    constructor.
+    + specialize (Hrel i).
+      now rewrite 2 lookup_insert in Hrel.
+    + apply IHm1.
+      intros j.
+      generalize (Hrel j).
+      rewrite 2 lookup_insert_case.
+      case_decide as Hij; [subst; now rewrite Hm1i, lookup_delete|].
+      done.
+Qed.
+
+
+(* The (strong) permutation relation on graphs, and its correctness *)
+
+Definition hg_strongperm_eq {T n m} (cohg cohg' : CospanHyperGraph T n m) : Prop :=
+  cohg.(inputs) = cohg'.(inputs) /\
+  cohg.(outputs) = cohg'.(outputs) /\
+  vertices cohg = vertices cohg' /\
+  map_relation (λ _ tio tio', abs_strongperm_eq tio tio')
+    (λ _ _, False) (λ _ _, False)
+    cohg.(hedges).(hyperedges) cohg'.(hedges).(hyperedges).
+
+Lemma graph_namedtensorlist_semantics_hg_strongperm_eq
+  {T n m} (cohg cohg' : CospanHyperGraph T n m) :
+  hg_strongperm_eq cohg cohg' ->
+  ntl_strongperm_eq (graph_namedtensorlist_semantics cohg)
+    (graph_namedtensorlist_semantics cohg').
+Proof.
+  intros (Hins & Houts & Hverts & Hperm).
+  apply map_relation_to_map_to_list in Hperm.
+  split; [|split].
+  - cbn.
+    now rewrite <- Hverts.
+  - cbn.
+    apply eqlistA_PermutationA, eqlistA_altdef.
+    unfold tg_abstracts.
+    apply Forall2_fmap.
+    eapply Forall2_impl; [apply Hperm|].
+    intros (k, tio) (k', tio').
+    cbn.
+    intros [<- Heq].
+    split; [done|].
+    cbn.
+    rewrite <- 2 fmap_app.
+    f_equiv.
+    apply Heq.
+  - cbn.
+    now rewrite <- Hins, Houts.
+Qed.
+
+Lemma graph_mabs_hg_strongperm_eq `{TensorLike R A T}
+  {n m} (cohg cohg' : CospanHyperGraph T n m) :
+  hg_strongperm_eq cohg cohg' ->
+  graph_mabs cohg.(hedges) = graph_mabs cohg'.(hedges).
+Proof.
+  intros (Hins & Houts & Hverts & Hperm).
+  unfold graph_mabs.
+  apply map_eq; intros i.
+  specialize (Hperm i).
+  rewrite 2 lookup_fmap.
+  destruct (_ !! _), (_ !! _); [|done..].
+  cbn in *.
+  now rewrite Hperm.1.
+Qed.
+
+Lemma hg_strongperm_eq_correct `{TensT : TensorLike R A T,
+  SR : SemiRing R rO rI radd rmul req,
+  !StronglyPermutativeTensorLike TensT,
+  SA : Summable A, EQA : EqDecision A}
+  {n m} (cohg cohg' : CospanHyperGraph T n m) :
+  hg_strongperm_eq cohg cohg' ->
+  graph_semantics (SR:=SR) cohg ≡ graph_semantics cohg'.
+Proof.
+  intros Hperm.
+  apply graph_mabs_hg_strongperm_eq in Hperm as Hmabs.
+  apply graph_namedtensorlist_semantics_hg_strongperm_eq in Hperm as Hntl.
+  intros v w Hv Hw.
+  cbn -[ntl_total_semantics].
+  unfold namedtensorlist_to_tensor.
+  rewrite <- Hmabs.
+  apply ntl_strongperm_eq_correct.
+  - apply graph_namedtensorlist_semantics_WF.
+  - done.
+  - intros i dt _ Hidt.
+    unfold graph_mabs in Hidt.
+    rewrite lookup_fmap in Hidt.
+    destruct (cohg.(hedges).(hyperedges) !! i); [|done].
+    revert Hidt.
+    intros [= <-].
+    apply interpretTensorStronglyPermutative.
+Qed.
+
+
