theories/TensorExpr/TEPerm.v
@@ -1,0 +1,451 @@
+Require Import Summable.
+Require StringCustomNotation.
+
+Require Import SetoidList SetoidPermutation.
+
+From stdpp Require Import strings fin_maps pmap gmap.
+From stdpp Require Import pretty.
+
+Require Import Aux_stdpp Aux_pos.
+
+#[local] Coercion pos_to_nat_pred : positive >-> nat.
+#[local] Coercion N.of_nat : nat >-> N.
+
+Local Open Scope positive_scope.
+Local Open Scope list_scope.
+
+Require Export TESyntax TESemantics TECospan.
+
+Section abs_strongperm_eq.
+
+Context {A B : Type}.
+
+Definition abs_strongperm_eq : relation (A * list B * list B) :=
+  fun flu flu' =>
+  flu.1.1 = flu'.1.1 /\
+  flu.1.2 ++ flu.2 ≡ₚ flu'.1.2 ++ flu'.2.
+
+Lemma abs_strongperm_eq_refl flu : abs_strongperm_eq flu flu.
+Proof.
+  easy.
+Qed.
+
+Lemma abs_strongperm_eq_symm flu flu' :
+  abs_strongperm_eq flu flu' -> abs_strongperm_eq flu' flu.
+Proof.
+  intros []; split; now symmetry.
+Qed.
+
+Lemma abs_strongperm_eq_trans flu flu' flu'' :
+  abs_strongperm_eq flu flu' -> abs_strongperm_eq flu' flu'' ->
+  abs_strongperm_eq flu flu''.
+Proof.
+  intros [] []; split; etransitivity; eauto.
+Qed.
+
+End abs_strongperm_eq.
+
+Add Parametric Relation {A B} : (A * list B * list B) (@abs_strongperm_eq A B)
+  reflexivity proved by abs_strongperm_eq_refl
+  symmetry proved by abs_strongperm_eq_symm
+  transitivity proved by abs_strongperm_eq_trans
+    as abs_strongperm_eq_setoid.
+
+
+Definition ntl_strongperm_eq (ntl ntl' : namedtensorlist) :=
+  ntl.(ntl_sums) ≡ₚ ntl'.(ntl_sums) /\
+  PermutationA abs_strongperm_eq ntl.(ntl_abstracts) ntl'.(ntl_abstracts) /\
+  PermutationA prod_swap_eq ntl.(ntl_deltas) ntl'.(ntl_deltas).
+
+Lemma ntl_strongperm_eq_refl ntl :
+  ntl_strongperm_eq ntl ntl.
+Proof.
+  easy.
+Qed.
+
+Lemma ntl_strongperm_eq_symm ntl ntl' :
+  ntl_strongperm_eq ntl ntl' -> ntl_strongperm_eq ntl' ntl.
+Proof.
+  intros (?&?&?); split; [|split]; now symmetry.
+Qed.
+
+Lemma ntl_strongperm_eq_trans ntl ntl' ntl'' :
+  ntl_strongperm_eq ntl ntl' -> ntl_strongperm_eq ntl' ntl'' ->
+  ntl_strongperm_eq ntl ntl''.
+Proof.
+  intros (?&?&?) (?&?&?); split; [|split]; now etransitivity; eauto.
+Qed.
+
+
+Add Parametric Relation : namedtensorlist ntl_strongperm_eq
+  reflexivity proved by ntl_strongperm_eq_refl
+  symmetry proved by ntl_strongperm_eq_symm
+  transitivity proved by ntl_strongperm_eq_trans
+    as ntl_strongperm_eq_setoid.
+
+
+
+
+Lemma deltas_vars_permA_mor :
+  Proper (PermutationA prod_swap_eq ==> eq) deltas_vars.
+Proof.
+  intros delt delt' Hdelt.
+  induction Hdelt as [|x y delt delt' Hx Hdelt| |];
+    [reflexivity| |set_solver|etransitivity; eassumption].
+  rewrite 2 deltas_vars_cons.
+  f_equiv; [|easy].
+  destruct Hx as [<- | <-]; [done|].
+  unfold_leibniz.
+  apply list_to_set_perm.
+  destruct x as []; cbn; solve_Permutation.
+Qed.
+
+
+Lemma abstracts_vars_cons flu abs :
+  abstracts_vars (flu :: abs) =
+  list_to_set (flu.1.2 ++ flu.2) ∪ abstracts_vars abs.
+Proof.
+  unfold abstracts_vars.
+  cbn.
+  destruct flu as [[]]; cbn.
+  apply list_to_set_app_L.
+Qed.
+
+Lemma abstracts_vars_permA_mor :
+  Proper (PermutationA abs_strongperm_eq ==> eq) abstracts_vars.
+Proof.
+  intros delt delt' Hdelt.
+  induction Hdelt as [|x y delt delt' Hx Hdelt| |];
+    [reflexivity| |set_solver|etransitivity; eassumption].
+  rewrite 2 abstracts_vars_cons.
+  f_equiv; [|easy].
+  apply list_to_set_perm_L, Hx.
+Qed.
+
+Lemma abstracts_bound_vars_permA_mor :
+  Proper (PermutationA abs_strongperm_eq ==> eq) abstracts_bound_vars.
+Proof.
+  intros delt delt' Hdelt.
+  rewrite <- 2 set_omap_v2bound_abstracts_vars.
+  f_equal.
+  now apply abstracts_vars_permA_mor.
+Qed.
+
+Lemma abstracts_free_vars_permA_mor :
+  Proper (PermutationA abs_strongperm_eq ==> eq) abstracts_free_vars.
+Proof.
+  intros delt delt' Hdelt.
+  rewrite <- 2 set_omap_v2free_abstracts_vars.
+  f_equal.
+  now apply abstracts_vars_permA_mor.
+Qed.
+
+Lemma ntl_varset_ntl_strongperm_eq ntl ntl' :
+  ntl_strongperm_eq ntl ntl' ->
+  ntl_varset ntl = ntl_varset ntl'.
+Proof.
+  unfold ntl_varset.
+  intros (_ & Habs & Hdelt).
+  f_equal.
+  - now apply abstracts_vars_permA_mor.
+  - now apply deltas_vars_permA_mor.
+Qed.
+
+Lemma ntl_free_varset_ntl_strongperm_eq ntl ntl' :
+  ntl_strongperm_eq ntl ntl' ->
+  ntl_free_varset ntl = ntl_free_varset ntl'.
+Proof.
+  unfold ntl_free_varset.
+  intros (_ & Habs & Hdelt).
+  f_equal.
+  - now apply abstracts_free_vars_permA_mor.
+  - now apply deltas_free_vars_permA_mor.
+Qed.
+
+Lemma ntl_bound_varset_ntl_strongperm_eq ntl ntl' :
+  ntl_strongperm_eq ntl ntl' ->
+  ntl_bound_varset ntl = ntl_bound_varset ntl'.
+Proof.
+  unfold ntl_bound_varset.
+  intros (_ & Habs & Hdelt).
+  f_equal.
+  - now apply abstracts_bound_vars_permA_mor.
+  - now apply deltas_bound_vars_permA_mor.
+Qed.
+
+Lemma ntl_strongperm_eq_WF ntl ntl' :
+  ntl_strongperm_eq ntl ntl' ->
+  WF_ntl ntl <-> WF_ntl ntl'.
+Proof.
+  rewrite 2 WF_ntl_alt_varset.
+  intros Heq.
+  apply ntl_bound_varset_ntl_strongperm_eq in Heq as Hvars.
+  rewrite <- Hvars.
+  rewrite <- Heq.1.
+  done.
+Qed.
+
+Lemma ntl_strongperm_eq_WT tl ntl ntl' :
+  ntl_strongperm_eq ntl ntl' ->
+  WT_ntl tl ntl <-> WT_ntl tl ntl'.
+Proof.
+  rewrite 2 WT_ntl_alt_varset.
+  intros Heq.
+  f_equiv; [|now apply ntl_strongperm_eq_WF].
+  now apply ntl_free_varset_ntl_strongperm_eq in Heq as <-.
+Qed.
+
+
+Definition abstracts_indices {A} (abs : list (Idx * list A * list A)) : Pset :=
+  list_to_set ((fst ∘ fst) <$> abs).
+
+Lemma abstracts_indices_ntl2tl ntl :
+  abstracts_indices (ntl2tl ntl).(tl_abstracts) =
+  abstracts_indices ntl.(ntl_abstracts).
+Proof.
+  destruct ntl as [isums abs].
+  cbn.
+  rewrite <- list_fmap_compose.
+  f_equal.
+  apply list_fmap_ext; now intros _ [[]] _.
+Qed.
+
+Lemma abstracts_indices_relabel_abs `(f : A -> B) abs :
+  abstracts_indices (relabel_abs f <$> abs) = abstracts_indices abs.
+Proof.
+  unfold abstracts_indices.
+  rewrite <- list_fmap_compose.
+  f_equal.
+  now apply list_fmap_ext; intros _ [[]] _.
+Qed.
+
+Lemma abstracts_indices_ntl_aeq ntl ntl' :
+  ntl =ntl= ntl' ->
+  abstracts_indices ntl.(ntl_abstracts) =
+  abstracts_indices ntl'.(ntl_abstracts).
+Proof.
+  intros (f & _ & _ & Habs & Hdelt).
+  unfold abstracts_indices.
+  rewrite <- Habs.
+  symmetry.
+  apply abstracts_indices_relabel_abs.
+Qed.
+
+Lemma abstracts_indices_relabel_absidx f ntl :
+  abstracts_indices (ntl_relabel_absidx f ntl).(ntl_abstracts) =
+  set_map f (abstracts_indices ntl.(ntl_abstracts)).
+Proof.
+  unfold abstracts_indices.
+  cbn.
+  rewrite <- list_fmap_compose.
+  unfold compose, prod_map; cbn.
+  rewrite set_map_list_to_set_L.
+  rewrite <- list_fmap_compose.
+  done.
+Qed.
+
+Lemma abstracts_indices_permA_mor {A} abs abs' :
+  PermutationA abs_strongperm_eq abs abs' ->
+  @abstracts_indices A abs = abstracts_indices abs'.
+Proof.
+  intros Hperm.
+  induction Hperm as [|x y delt delt' Hx Hdelt| |];
+    [reflexivity| |set_solver|etransitivity; eassumption].
+  cbn -[union].
+  f_equiv; [|easy].
+  now rewrite Hx.1.
+Qed.
+
+Section ntl_strongperm_eq_corr.
+
+Local Open Scope nat_scope.
+
+Import Tensor.
+
+Context `{SR : SemiRing R rO rI radd rmul req}.
+
+Notation "0" := rO.
+Notation "1" := rI.
+Notation "x '==' y" := (req x y) (at level 70).
+Infix "+" := radd.
+Infix "*" := rmul.
+
+Add Ring R : SR.(RSRth)
+  (setoid SR.(Req_equiv) SR.(Req_ext)).
+
+Let Req_equivalence : Equivalence req := Req_equiv.
+Local Existing Instance Req_equivalence.
+
+Let Radd_proper := Req_ext.(SRadd_ext) : Proper (req ==> req ==> req) radd.
+Local Existing Instance Radd_proper.
+
+Let Rmul_proper := Req_ext.(SRmul_ext) : Proper (req ==> req ==> req) rmul.
+Local Existing Instance Rmul_proper.
+
+Context `{SA : Summable A, AEQ : EqDecision A}.
+
+
+Lemma tl_total_semantics_aux_absidxs_ext
+  mabs mabs' ml mr sums abs delt :
+  (forall i, i ∈ abstracts_indices abs -> mabs !! i = mabs' !! i) ->
+  req (tl_total_semantics_aux (SR:=SR) mabs ml mr sums abs delt)
+    (tl_total_semantics_aux mabs' ml mr sums abs delt).
+Proof.
+  intros Habs.
+  revert mr;
+  induction sums; intros mr;
+  [|cbn; apply sum_of_ext; intros ?; apply IHsums].
+  apply tl_total_semantics_aux_ext_base; apply Forall_Forall2_diag;
+  rewrite Forall_forall.
+  - intros [[f low] up] Hflu.
+    split; [|split; apply Forall_Forall2_diag;
+      rewrite Forall_forall; intros; reflexivity].
+    cbn.
+    apply Habs.
+    set_unfold.
+    now exists (f, low, up).
+  - easy.
+Qed.
+
+Lemma ntl_total_semantics_absidxs_ext
+  mabs mabs' ml ntl :
+  (forall i, i ∈ abstracts_indices ntl.(ntl_abstracts) -> mabs !! i = mabs' !! i) ->
+  req (ntl_total_semantics (SR:=SR) mabs ml ntl)
+    (ntl_total_semantics mabs' ml ntl).
+Proof.
+  intros Habs.
+  apply tl_total_semantics_aux_absidxs_ext.
+  destruct ntl as [isums abs delt].
+  rewrite abstracts_indices_ntl2tl.
+  apply Habs.
+Qed.
+
+
+Lemma ntl_total_semantics_relabel_free
+  f `{Hf : !Inj eq eq f} mabs ml ntl :
+  req (ntl_total_semantics (SR:=SR) mabs (kmap f ml) (ntl_relabel_free f ntl))
+    (ntl_total_semantics mabs ml ntl).
+Proof.
+  unfold ntl_total_semantics.
+  rewrite ntl2tl_ntl_relabel_free.
+  apply (relabel_tl_free_semantics_aux_kmap _).
+Qed.
+
+Lemma abstracts_semantics_alt_cons mabs ml mr flu abs :
+  abstracts_semantics_alt mabs ml mr (flu :: abs) =
+  abstract_semantics_alt (rO:=rO) mabs ml mr flu.1.1 flu.1.2 flu.2 *
+  abstracts_semantics_alt (A:=A) mabs ml mr abs.
+Proof.
+  now destruct flu as [[]].
+Qed.
+
+Lemma deltas_semantics_alt_cons ml mr lu delt :
+  deltas_semantics_alt ml mr (lu :: delt) =
+  delta_semantics_alt (rO:=rO) ml mr lu.1 lu.2 *
+  deltas_semantics_alt (A:=A) ml mr delt.
+Proof.
+  now destruct lu as [].
+Qed.
+
+Lemma abstract_semantics_alt_to_app mabs ml mr f low up :
+  abstract_semantics_alt (rO:=rO) (A:=A) mabs ml mr f low up =
+  default 0 (lrargs ← join_list (get_var_alt ml mr <$> (low ++ up));
+    dt ← mabs !! f;
+    Some $ Vapplys dt (take (length low) lrargs) (drop (length low) lrargs)).
+Proof.
+  unfold abstract_semantics_alt.
+  rewrite fmap_app, join_list_app, option_bind_assoc'.
+  destruct (join_list (_ <$> low)) as [largs|] eqn:Hlargs; [cbn|done].
+  rewrite option_fmap_bind; unfold compose; cbn.
+  destruct (join_list (_ <$> up)) as [uargs|] eqn:Huargs; [cbn|done].
+  destruct (mabs !! f) as [dt|]; [cbn|done].
+  apply join_list_Some_length in Hlargs.
+  rewrite length_fmap in Hlargs.
+  f_equal; symmetry;
+  [etransitivity; [|apply take_app_length]|
+   etransitivity; [|apply drop_app_length]]; now f_equal.
+Qed.
+
+
+Lemma abs_strongperm_eq_correct_sem mabs ml mr
+  (abs abs' : positive * list var * list var) :
+  abs_strongperm_eq abs abs' ->
+  (forall dt, mabs !! abs.1.1 = Some dt -> strongly_permutative_tensor (A:=A) dt) ->
+  abstract_semantics_alt (rO:=rO) mabs ml mr abs.1.1 abs.1.2 abs.2 ==
+  abstract_semantics_alt (rO:=rO) mabs ml mr abs'.1.1 abs'.1.2 abs'.2.
+Proof.
+  intros [<- Hperm] Hsp.
+  rewrite 2 abstract_semantics_alt_to_app.
+  destruct (mabs !! abs.1.1) as [ma|] eqn:Hma; [|cbn; now rewrite !option_bind_None_r].
+  specialize (Hsp _ eq_refl).
+  apply (fmap_Permutation (get_var_alt ml mr)) in Hperm as Hperm'%join_list_Permutation.
+  induction Hperm as [lrargs lrargs' Hlrargs|]; [|done].
+  cbn.
+  apply Hsp.
+  rewrite 4 vec_to_list_to_vec.
+  now rewrite 2 take_drop.
+Qed.
+
+Lemma abstracts_semantics_alt_permA mabs ml mr 
+  (abs abs' : list (positive * list var * list var)) :
+  PermutationA abs_strongperm_eq abs abs' ->
+  (forall i dt, i ∈ abstracts_indices abs -> mabs !! i = Some dt ->
+    strongly_permutative_tensor (A:=A) dt) ->
+  abstracts_semantics_alt mabs ml mr abs == 
+  abstracts_semantics_alt mabs ml mr abs'.
+Proof.
+  intros Hperm Hsp.
+  pose proof (fun l1 l2 H => (eq_reflexivity _ _
+    (eq_sym (abstracts_indices_permA_mor (A:=var) l1 l2 H))) : _ ⊆ _) as Hsub.
+  unfold subseteq, set_subseteq_instance in Hsub.
+  induction Hperm as [|x y delt delt' Hx Hdelt| |];
+    [reflexivity| |rewrite 4 abstracts_semantics_alt_cons; ring|etransitivity; eauto].
+  rewrite 2 abstracts_semantics_alt_cons.
+  f_equiv; [|apply IHHdelt; intros ? ? Hin; apply Hsp; set_solver + Hin].
+  apply abs_strongperm_eq_correct_sem; [done|].
+  intros ?; apply Hsp.
+  cbn -[union].
+  now apply union_subseteq_l, elem_of_singleton.
+Qed.
+
+Lemma deltas_semantics_alt_permA ml mr (delt delt' : list (var * var)) : 
+  PermutationA prod_swap_eq delt delt' ->
+  deltas_semantics_alt ml mr delt == deltas_semantics_alt (A:=A) ml mr delt'.
+Proof.
+  intros Hdelt.
+  unfold deltas_semantics_alt.
+  apply Rlist_prod_perm_mor.
+  induction Hdelt as [|? ? ? ? Heq | |].
+  - done.
+  - cbn.
+    f_equiv; [|easy].
+    do 2 case_match.
+    rewrite prod_swap_eq_pair in Heq.
+    destruct Heq as [[-> ->]|[-> ->]]; [done|].
+    apply eq_reflexivity, delta_semantics_alt_comm.
+  - apply (Permutation_PermutationA _).
+    solve_Permutation.
+  - now etransitivity; eassumption.
+Qed.
+
+Lemma ntl_strongperm_eq_correct mabs ml (ntl ntl' : namedtensorlist) :
+  WF_ntl ntl ->
+  ntl_strongperm_eq ntl ntl' ->
+  (forall i dt, i ∈ abstracts_indices ntl.(ntl_abstracts) -> mabs !! i = Some dt ->
+    strongly_permutative_tensor dt) ->
+  ntl_total_semantics mabs ml ntl ==
+  ntl_total_semantics mabs ml ntl'.
+Proof.
+  intros Hwf Heq Hperm.
+  pose proof Hwf as Hwf'.
+  erewrite ntl_strongperm_eq_WF in Hwf' by eassumption.
+  rewrite 2 ntl_total_semantics_alt by done.
+  erewrite <- (sum_of_Vmap_perm _ _ _ Heq.1).
+  apply sum_of_ext'; intros mr Hmr%elem_of_Vmap_elements_1.
+  f_equiv.
+  - apply abstracts_semantics_alt_permA, Hperm.
+    apply Heq.
+  - apply deltas_semantics_alt_permA, Heq.
+Qed.
+
+End ntl_strongperm_eq_corr.
